Added some loop combinators (some admits left)

ulib/LowStar.RST.Loops.fst
@@ -1,7 +1,236 @@
 module LowStar.RST.Loops
 
+
+module R = LowStar.Resource
+module RST = LowStar.RST
+module A = LowStar.Array
+module AR = LowStar.RST.Array
+module HS = FStar.HyperStack
+module HST = FStar.HyperStack.ST
+module L = C.Loops
+module P = LowStar.Permissions
+
+open FStar.Mul
+
 let rec while res inv guard test body =
   if test () then begin
     body ();
     while res inv guard test body
   end
+
+
+val for:
+  start:U32.t ->
+  finish:U32.t{U32.v finish >= U32.v start} ->
+  context:R.resource ->
+  inv:(h:R.imem (R.inv context) -> nat -> Type0) ->
+  f:(i:U32.t{U32.(v start <= v i /\ v i < v finish)} -> RST unit
+    (context)
+    (fun _ -> context)
+    (requires (fun h -> inv h (U32.v i)))
+    (ensures (fun h_1 _ h_2 -> U32.(inv h_1 (v i) /\ inv h_2 (v i + 1))))
+  ) ->
+  RST unit
+    (context)
+    (fun _ -> context)
+    (requires (fun h -> inv h (U32.v start)))
+    (ensures (fun _ _ h_2 -> inv h_2 (U32.v finish)))
+
+let rec for start finish inv context f =
+  if start = finish then
+    ()
+  else begin
+    f start;
+    for (U32.(start +^ 1ul)) finish inv context f
+  end
+
+val for_each:
+  #a: Type ->
+  #context: resource ->
+  b: A.array a ->
+  #inv:(h:R.imem (R.inv context) -> i:nat -> Type) ->
+  f: (i:U32.t{U32.v i < A.vlength b} -> x:a -> RST unit
+    (context)
+    (fun _ -> context)
+    (fun h0 -> inv h0 (U32.v i) /\ x == Seq.index (A.as_seq h0 b) (U32.v i))
+    (fun h0 _ h1 -> inv h0 (U32.v i) /\ inv h1 (U32.v i + 1))
+  ) ->
+  RST unit
+    (R.(context <*> AR.array_resource b))
+    (fun _ -> R.(context <*> AR.array_resource b))
+    (fun h0 -> inv h0 0)
+    (fun h0 _ h1 -> inv h1 (A.vlength b) /\
+      R.sel (R.view_of (AR.array_resource b)) h0 ==
+      R.sel (R.view_of (AR.array_resource b)) h1
+    )
+
+let for_each #a #context b #inv f =
+  (**) let hinit = HST.get () in
+  (**) let correct_inv = fun h i -> inv h i /\
+  (**)  R.sel (R.view_of (AR.array_resource b)) hinit ==
+  (**)  R.sel (R.view_of (AR.array_resource b)) h
+  (**) in
+  let correct_f (i:U32.t{U32.(0 <= v i /\ v i < A.vlength b)})
+    : RST unit
+      (R.(context <*> AR.array_resource b))
+      (fun _ -> R.(context <*> AR.array_resource b))
+      (requires (fun h0 ->
+        correct_inv h0 (U32.v i)
+      ))
+      (ensures (fun h0 _ h1 ->
+        U32.(correct_inv h0 (v i) /\ correct_inv h1 (v i + 1))
+      ))
+   =
+     let x = RST.rst_frame
+       (R.(context <*> AR.array_resource b))
+       (fun _ -> R.(context <*> AR.array_resource b))
+       (fun _ -> AR.index b i)
+     in
+     admit();
+     RST.rst_frame
+       (R.(context <*> AR.array_resource b))
+       #context
+       (fun _ -> R.(context <*> AR.array_resource b))
+       #(fun _ -> context)
+       #(AR.array_resource b)
+       #(fun h0 -> inv h0 (U32.v i) /\ x == Seq.index (A.as_seq h0 b) (U32.v i))
+       #(fun h0 _ h1 -> inv h0 (U32.v i) /\ inv h1 (U32.v i + 1))
+       (fun _ -> let f' = f i x in f')
+  in
+  for
+    0ul
+    (A.length b)
+    (R.(context <*> AR.array_resource b))
+    correct_inv
+    correct_f
+
+val mapi:
+  #a: Type ->
+  #a': Type ->
+  #context: resource ->
+  output: A.array a' ->
+  input: A.array a{A.length output = A.length input} ->
+  #spec_f:(i:nat -> a -> GTot a') ->
+  f: (i:U32.t{U32.v i < A.vlength input} -> x:a -> RST a'
+    (context)
+    (fun _ -> context)
+    (fun h0 -> x == Seq.index (A.as_seq h0 input) (U32.v i))
+    (fun h0 y h1 -> y == spec_f (U32.v i) x)
+  ) ->
+  RST unit
+    (R.(context <*> AR.array_resource output <*> AR.array_resource input))
+    (fun _ -> R.(context <*> AR.array_resource output <*> AR.array_resource input))
+    (fun h0 -> P.allows_write (R.sel (R.view_of (AR.array_resource output)) h0).AR.p)
+    (fun h0 _ h1 ->
+      R.sel (R.view_of (AR.array_resource input)) h1 ==
+      R.sel (R.view_of (AR.array_resource input)) h0 /\
+      (R.sel (R.view_of (AR.array_resource output)) h1).AR.p =
+      (R.sel (R.view_of (AR.array_resource output)) h0).AR.p /\
+      (R.sel (R.view_of (AR.array_resource output)) h1).AR.s ==
+      Seq.init_ghost (A.vlength output) (fun i ->
+        spec_f i (Seq.index (R.sel (R.view_of (AR.array_resource input)) h0).AR.s i)
+      )
+    )
+
+let mapi #a #a' #context output input #spec_f f =
+  (**) let hinit = HST.get () in
+  (**) let correct_context = R.(context <*> AR.array_resource output) in
+  (**) let correct_inv (h:R.imem (R.inv correct_context)) (i:nat) : Type =
+  (**)   let i = if i >= A.vlength input then A.vlength input else i in
+  (**)   (R.sel (R.view_of (AR.array_resource output)) h).AR.p =
+  (**)   (R.sel (R.view_of (AR.array_resource output)) hinit).AR.p /\
+  (**)   Seq.slice (R.sel (R.view_of (AR.array_resource output)) h).AR.s 0 i ==
+  (**)   Seq.init_ghost i (fun j ->
+  (**)     spec_f j (Seq.index (R.sel (R.view_of (AR.array_resource input)) hinit).AR.s j)
+  (**)   )
+  in
+  let correct_f (i:U32.t{U32.v i < A.vlength input}) (x:a) : RST unit
+    (R.(context <*> AR.array_resource output))
+    (fun _ -> R.(context <*> AR.array_resource output))
+    (fun h0 -> correct_inv h0 (U32.v i) /\ x == Seq.index (A.as_seq h0 input) (U32.v i))
+    (fun h0 _ h1 -> correct_inv h0 (U32.v i) /\ correct_inv h1 (U32.v i + 1))
+  =
+   (**) let h0 = HST.get () in
+    let new_x = RST.rst_frame
+      (R.(context <*> AR.array_resource output))
+      (fun _ -> R.(context <*> AR.array_resource output))
+      (fun _ -> f i x)
+    in
+    RST.rst_frame
+      (R.(context <*> AR.array_resource output))
+      (fun _ -> R.(context <*> AR.array_resource output))
+      (fun _ -> AR.upd output i new_x);
+    (**) let h1 = HST.get () in
+    (**) assert(correct_inv h0 (U32.v i));
+    (**) if U32.v i >= A.vlength input then
+    (**)   ()
+    (**) else begin
+    (**)   let vi = if U32.v i >= A.vlength input then A.vlength input else U32.v i in
+    (**)   assert(vi = U32.v i);
+    (**)   assert(Seq.slice (R.sel (R.view_of (AR.array_resource output)) h1).AR.s 0 vi ==
+    (**)     Seq.init_ghost vi (fun j ->
+    (**)       spec_f j (Seq.index (R.sel (R.view_of (AR.array_resource input)) hinit).AR.s j)
+    (**)     )
+    (**)   );
+    (**)  let vi_plus_one = if U32.v i + 1 >= A.vlength input then A.vlength input else U32.v i + 1 in
+    (**)  let aux (j:nat{j < vi_plus_one}) : Lemma (
+    (**)    Seq.index (Seq.slice (R.sel (R.view_of (AR.array_resource output)) h1).AR.s 0 vi_plus_one) j ==
+    (**)    Seq.index
+    (**)      (Seq.init_ghost vi_plus_one
+    (**)        (fun j' -> spec_f j' (Seq.index (R.sel (R.view_of (AR.array_resource input)) hinit).AR.s j')))
+    (**)    j
+    (**)  ) =
+    (**)    assert(
+    (**)      Seq.index (Seq.slice (R.sel (R.view_of (AR.array_resource output)) h1).AR.s 0 vi_plus_one) j ==
+    (**)      Seq.index (R.sel (R.view_of (AR.array_resource output)) h1).AR.s j
+    (**)    );
+    (**)    assert(
+    (**)      Seq.index
+    (**)        (Seq.init_ghost vi_plus_one
+    (**)          (fun j' -> spec_f j' (Seq.index (R.sel (R.view_of (AR.array_resource input)) hinit).AR.s j')))
+    (**)      j  ==
+    (**)      spec_f j (Seq.index (R.sel (R.view_of (AR.array_resource input)) hinit).AR.s j)
+    (**)    );
+    (**)    if j = U32.v i then begin
+    (**)      assert(Seq.index (Seq.slice (R.sel (R.view_of (AR.array_resource output)) h1).AR.s 0 vi_plus_one) j ==
+    (**)        Seq.index (R.sel (R.view_of (AR.array_resource output)) h1).AR.s j
+    (**)      );
+    (**)      assert(Seq.index
+    (**)        (Seq.init_ghost vi_plus_one
+    (**)          (fun j' -> spec_f j' (Seq.index (R.sel (R.view_of (AR.array_resource input)) hinit).AR.s j')))
+    (**)          j ==
+    (**)          spec_f j (Seq.index (R.sel (R.view_of (AR.array_resource input)) hinit).AR.s j)
+    (**)      );
+    (**)     assert(
+    (**)       Seq.index (R.sel (R.view_of (AR.array_resource output)) h1).AR.s j ==
+    (**)       new_x
+    (**)     );
+    (**)     admit();
+    (**)     assert( Seq.index (R.sel (R.view_of (AR.array_resource input)) h0).AR.s j ==
+    (**)        Seq.index (R.sel (R.view_of (AR.array_resource input)) hinit).AR.s j);
+    (**)     admit()
+    (**)    end else begin
+    (**)      assert(Seq.index (R.sel (R.view_of (AR.array_resource output)) h1).AR.s j ==
+    (**)        Seq.index (R.sel (R.view_of (AR.array_resource output)) h0).AR.s j);
+    (**)      assert(Seq.slice (R.sel (R.view_of (AR.array_resource output)) h0).AR.s 0 vi ==
+    (**)        Seq.init_ghost vi (fun j' ->
+    (**)          spec_f j' (Seq.index (R.sel (R.view_of (AR.array_resource input)) hinit).AR.s j')
+    (**)      ));
+    (**)      assert(Seq.index (Seq.slice (R.sel (R.view_of (AR.array_resource output)) h0).AR.s 0 vi) j ==
+    (**)        Seq.index (R.sel (R.view_of (AR.array_resource output)) h0).AR.s j
+    (**)      );
+    (**)      assert(Seq.index (R.sel (R.view_of (AR.array_resource output)) h0).AR.s j ==
+    (**)        spec_f j (Seq.index (R.sel (R.view_of (AR.array_resource input)) hinit).AR.s j)
+    (**)      )
+    (**)    end
+    (**)  in
+    (**)  Classical.forall_intro aux;
+    (**)  assert(Seq.slice (R.sel (R.view_of (AR.array_resource output)) h1).AR.s 0 vi_plus_one `Seq.equal`
+    (**)     Seq.init_ghost vi_plus_one (fun j ->
+    (**)       spec_f j (Seq.index (R.sel (R.view_of (AR.array_resource input)) hinit).AR.s j)
+    (**)     )
+    (**)   )
+    (**) end
+  in
+  admit();
+  for_each #a #R.(context <*> AR.array_resource output) input #correct_inv correct_f
